src/Bedrock/Field/Synthesis/Examples/p224_64_new.v
@@ -48,7 +48,7 @@ Section Field.
   Require Import bedrock2.BasicC32Semantics.
 
   (* Call fiat-crypto pipeline on all field operations *)
-  Instance p224_ops : @word_by_word_Montgomery_ops from_mont_string to_mont_string _ _ _ _ _ _ _ _ _ _ (WordByWordMontgomery.n m machine_wordsize) m.
+  Instance p224_ops : @word_by_word_Montgomery_ops from_mont_string to_mont_string _ _ _ _ _ _ _ _ _ (WordByWordMontgomery.n m machine_wordsize) m.
   Proof using Type. Time constructor; make_computed_op. Defined.
 
   Instance frep224 : FieldRepresentation := field_representation m.
