src/Bedrock/Field/Translation/Proofs/ValidComputable/Func.v
@@ -2,8 +2,9 @@ From Coq Require Import ZArith.
 From Coq Require Import Bool.
 From Coq Require Import List.
 From Coq Require Import Lia.
+Require Import coqutil.Word.Bitwidth.
 Require Import bedrock2.Syntax.
-Require Import coqutil.Word.Interface coqutil.Word.Properties.
+Require Import coqutil.Word.Properties.
 Require Import coqutil.Map.Interface.
 Require Import Crypto.Bedrock.Field.Common.Types.
 Require Import Crypto.Bedrock.Field.Common.Tactics.
@@ -24,8 +25,9 @@ Import Types.Notations.
 
 Section Func.
   Context
-    {width BW word mem locals ext_spec varname_gen error}
-   `{parameters_sentinel : @parameters width BW word mem locals ext_spec varname_gen error}.
+    {width BW mem locals ext_spec varname_gen error}
+   `{parameters_sentinel : @parameters width BW mem locals ext_spec varname_gen error}.
+  Local Notation word := (bits width).
   Context {ok : ok }.
   Local Existing Instance Types.rep.Z.
 
